WIP

src/ModSimStutter.v
@@ -4,8 +4,8 @@ Require Export Coq.Strings.String.
 Require Import Coq.Classes.RelationClasses.
 
 From Fairness Require Export ITreeLib FairBeh Mod.
-From Fairness Require Import pind.
-From Fairness Require Import PCM.
+From Fairness Require Import pind PCM.
+From Fairness Require Import ModSimNoSync.
 
 Set Implicit Arguments.
 
@@ -44,16 +44,17 @@ Section PRIMIVIESIM.
 
   Variant __lsim
           (tid: thread_id)
-          (lsim: forall R_src R_tgt (RR: R_src -> R_tgt -> URA.car -> wf_stt.(T) -> shared_rel), bool -> bool -> URA.car -> (wf_stt.(T) * itree srcE R_src) -> itree tgtE R_tgt -> shared_rel)
-          (_lsim: forall R_src R_tgt (RR: R_src -> R_tgt -> URA.car -> wf_stt.(T) -> shared_rel),bool -> bool -> URA.car -> (wf_stt.(T) * itree srcE R_src) -> itree tgtE R_tgt -> shared_rel)
-          R_src R_tgt (RR: R_src -> R_tgt -> URA.car -> wf_stt.(T) -> shared_rel)
+          (lsim: forall R_src R_tgt (RR: R_src -> R_tgt -> URA.car -> shared_rel), bool -> bool -> URA.car -> (wf_stt.(T) * itree srcE R_src) -> itree tgtE R_tgt -> shared_rel)
+          (_lsim: forall R_src R_tgt (RR: R_src -> R_tgt -> URA.car -> shared_rel),bool -> bool -> URA.car -> (wf_stt.(T) * itree srcE R_src) -> itree tgtE R_tgt -> shared_rel)
+          R_src R_tgt (RR: R_src -> R_tgt -> URA.car -> shared_rel)
     :
     bool -> bool -> URA.car -> (wf_stt.(T) * itree srcE R_src) -> itree tgtE R_tgt -> shared_rel :=
   | lsim_ret
-      f_src f_tgt r_ctx o
+      f_src f_tgt r_ctx o o0
       ths im_src im_tgt st_src st_tgt r_shared
       r_src r_tgt
-      (LSIM: RR r_src r_tgt r_ctx o (ths, im_src, im_tgt, st_src, st_tgt, r_shared))
+      (LT: wf_stt.(lt) o0 o)
+      (LSIM: RR r_src r_tgt r_ctx (ths, im_src, im_tgt, st_src, st_tgt, r_shared))
     :
     __lsim tid lsim _lsim RR f_src f_tgt r_ctx (o, Ret r_src) (Ret r_tgt) (ths, im_src, im_tgt, st_src, st_tgt, r_shared)
 
@@ -193,13 +194,21 @@ Section PRIMIVIESIM.
       r_ctx o
       ths im_src im_tgt st_src st_tgt r_shared
       itr_src itr_tgt
-      (LSIM: lsim _ _ RR false false r_ctx (o, itr_src) itr_tgt (ths, im_src, im_tgt, st_src, st_tgt, r_shared))
+      (LSIM: ModSimNoSync.lsim I tid RR false false r_ctx itr_src itr_tgt (ths, im_src, im_tgt, st_src, st_tgt, r_shared))
     :
     __lsim tid lsim _lsim RR true true r_ctx (o, itr_src) itr_tgt (ths, im_src, im_tgt, st_src, st_tgt, r_shared)
+
+  (* | lsim_progress *)
+  (*     r_ctx o *)
+  (*     ths im_src im_tgt st_src st_tgt r_shared *)
+  (*     itr_src itr_tgt *)
+  (*     (LSIM: lsim _ _ RR false false r_ctx (o, itr_src) itr_tgt (ths, im_src, im_tgt, st_src, st_tgt, r_shared)) *)
+  (*   : *)
+  (*   __lsim tid lsim _lsim RR true true r_ctx (o, itr_src) itr_tgt (ths, im_src, im_tgt, st_src, st_tgt, r_shared) *)
   .
 
   Definition lsim (tid: thread_id)
-             R_src R_tgt (RR: R_src -> R_tgt -> URA.car -> wf_stt.(T) -> shared_rel):
+             R_src R_tgt (RR: R_src -> R_tgt -> URA.car -> shared_rel):
     bool -> bool -> URA.car -> (wf_stt.(T) * itree srcE R_src) -> itree tgtE R_tgt -> shared_rel :=
     paco9 (fun r => pind9 (__lsim tid r) top9) bot9 R_src R_tgt RR.
 
@@ -226,8 +235,8 @@ Section PRIMIVIESIM.
   Qed.
 
   Variant lsim_resetC
-          (r: forall R_src R_tgt (RR: R_src -> R_tgt -> URA.car -> wf_stt.(T) -> shared_rel), bool -> bool -> URA.car -> (wf_stt.(T) * itree srcE R_src) -> itree tgtE R_tgt -> shared_rel)
-          R_src R_tgt (RR: R_src -> R_tgt -> URA.car -> wf_stt.(T) -> shared_rel)
+          (r: forall R_src R_tgt (RR: R_src -> R_tgt -> URA.car -> shared_rel), bool -> bool -> URA.car -> (wf_stt.(T) * itree srcE R_src) -> itree tgtE R_tgt -> shared_rel)
+          R_src R_tgt (RR: R_src -> R_tgt -> URA.car -> shared_rel)
     :
     bool -> bool -> URA.car -> (wf_stt.(T) * itree srcE R_src) -> itree tgtE R_tgt -> shared_rel :=
     | lsim_resetC_intro
@@ -250,7 +259,7 @@ Section PRIMIVIESIM.
     { ii. inv IN. econs; eauto. }
     i. inv PR. eapply GF in REL.
     eapply pind9_acc in REL.
-    instantiate (1:= (fun R0 R1 (RR: R0 -> R1 -> URA.car -> wf_stt.(T) -> shared_rel) ps1 pt1 r_ctx src tgt shr =>
+    instantiate (1:= (fun R0 R1 (RR: R0 -> R1 -> URA.car -> shared_rel) ps1 pt1 r_ctx src tgt shr =>
                         forall ps0 pt0,
                           (ps1 = true -> ps0 = true) ->
                           (pt1 = true -> pt0 = true) ->
@@ -324,13 +333,13 @@ Section PRIMIVIESIM.
       destruct LSIM as [LSIM IND]. hexploit IH; eauto.
     }
 
-    { pclearbot. hexploit H; ss; i. hexploit H0; ss; i. clarify.
-      eapply pind9_fold. eapply lsim_progress. eapply rclo9_base. auto. }
+    { hexploit H; ss; i. hexploit H0; ss; i. clarify.
+      eapply pind9_fold. eapply lsim_progress. auto. }
   Qed.
 
   Lemma lsim_reset_prog
         tid
-        R0 R1 (RR: R0 -> R1 -> URA.car -> wf_stt.(T) -> shared_rel)
+        R0 R1 (RR: R0 -> R1 -> URA.car -> shared_rel)
         src tgt shr
         ps0 pt0 ps1 pt1 r_ctx
         (LSIM: lsim tid RR ps1 pt1 r_ctx src tgt shr)
@@ -349,118 +358,127 @@ Section PRIMIVIESIM.
     right. auto.
   Qed.
 
-  Lemma lsim_set_prog
-        tid
-        R0 R1 (RR: R0 -> R1 -> URA.car -> wf_stt.(T) -> shared_rel)
-        r_ctx src tgt shr
-        (LSIM: lsim tid RR true true r_ctx src tgt shr)
-    :
-    forall ps pt, lsim tid RR ps pt r_ctx src tgt shr.
-  Proof.
-    i. revert_until tid. pcofix CIH. i.
-    remember true as ps0 in LSIM at 1. remember true as pt0 in LSIM at 1.
-    move LSIM before CIH. revert_until LSIM. punfold LSIM.
-    2:{ eapply lsim_mon. }
-    eapply pind9_acc in LSIM.
+  (* Lemma lsim_set_prog *)
+  (*       tid *)
+  (*       R0 R1 (RR: R0 -> R1 -> URA.car -> shared_rel) *)
+  (*       r_ctx src tgt shr *)
+  (*       (LSIM: lsim tid RR true true r_ctx src tgt shr) *)
+  (*   : *)
+  (*   forall ps pt, lsim tid RR ps pt r_ctx src tgt shr. *)
+  (* Proof. *)
+  (*   i. revert_until tid. pcofix CIH. i. *)
+  (*   remember true as ps0 in LSIM at 1. remember true as pt0 in LSIM at 1. *)
+  (*   move LSIM before CIH. revert_until LSIM. punfold LSIM. *)
+  (*   2:{ eapply lsim_mon. } *)
+  (*   eapply pind9_acc in LSIM. *)
 
-    { instantiate (1:= (fun R0 R1 (RR: R0 -> R1 -> URA.car -> wf_stt.(T) -> shared_rel) ps0 pt0 r_ctx src tgt shr =>
-                          ps0 = true ->
-                          pt0 = true ->
-                          forall ps pt,
-                            paco9
-                              (fun r0 =>
-                                 pind9 (__lsim tid r0) top9) r R0 R1 RR ps pt r_ctx src tgt shr)) in LSIM; auto. }
+  (*   { instantiate (1:= (fun R0 R1 (RR: R0 -> R1 -> URA.car -> shared_rel) ps0 pt0 r_ctx src tgt shr => *)
+  (*                         ps0 = true -> *)
+  (*                         pt0 = true -> *)
+  (*                         forall ps pt, *)
+  (*                           paco9 *)
+  (*                             (fun r0 => *)
+  (*                                pind9 (__lsim tid r0) top9) r R0 R1 RR ps pt r_ctx src tgt shr)) in LSIM; auto. } *)
 
-    ss. clear ps0 pt0 r_ctx src tgt shr LSIM.
-    intros rr DEC IH R0' R1' RR' gps gpt r_ctx src tgt shr LSIM. clear DEC.
-    intros Egps Egpt ps pt.
-    eapply pind9_unfold in LSIM.
-    2:{ eapply _lsim_mon. }
-    inv LSIM.
+  (*   ss. clear ps0 pt0 r_ctx src tgt shr LSIM. *)
+  (*   intros rr DEC IH R0' R1' RR' gps gpt r_ctx src tgt shr LSIM. clear DEC. *)
+  (*   intros Egps Egpt ps pt. *)
+  (*   eapply pind9_unfold in LSIM. *)
+  (*   2:{ eapply _lsim_mon. } *)
+  (*   inv LSIM. *)
 
-    { pfold. eapply pind9_fold. econs; eauto. }
+  (*   { pfold. eapply pind9_fold. econs; eauto. } *)
 
-    { destruct LSIM0 as [LSIM0 IND]. clear LSIM0.
-      pfold. eapply pind9_fold. eapply lsim_tauL. split; ss.
-      hexploit IH. eauto. all: eauto. i. punfold H. eapply lsim_mon.
-    }
+  (*   { destruct LSIM0 as [LSIM0 IND]. clear LSIM0. *)
+  (*     pfold. eapply pind9_fold. eapply lsim_tauL. split; ss. *)
+  (*     hexploit IH. eauto. all: eauto. i. punfold H. eapply lsim_mon. *)
+  (*   } *)
 
-    { des. pfold. eapply pind9_fold. eapply lsim_chooseL. esplits; eauto. split; ss.
-      destruct LSIM0 as [LSIM0 IND]. hexploit IH; eauto. i. punfold H. eapply lsim_mon.
-    }
+  (*   { des. pfold. eapply pind9_fold. eapply lsim_chooseL. esplits; eauto. split; ss. *)
+  (*     destruct LSIM0 as [LSIM0 IND]. hexploit IH; eauto. i. punfold H. eapply lsim_mon. *)
+  (*   } *)
 
-    { pfold. eapply pind9_fold. eapply lsim_putL. split; ss.
-      destruct LSIM0 as [LSIM0 IND]. hexploit IH; eauto. i. punfold H. eapply lsim_mon.
-    }
+  (*   { pfold. eapply pind9_fold. eapply lsim_putL. split; ss. *)
+  (*     destruct LSIM0 as [LSIM0 IND]. hexploit IH; eauto. i. punfold H. eapply lsim_mon. *)
+  (*   } *)
 
-    { pfold. eapply pind9_fold. eapply lsim_getL. split; ss.
-      destruct LSIM0 as [LSIM0 IND]. hexploit IH; eauto. i. punfold H. eapply lsim_mon.
-    }
+  (*   { pfold. eapply pind9_fold. eapply lsim_getL. split; ss. *)
+  (*     destruct LSIM0 as [LSIM0 IND]. hexploit IH; eauto. i. punfold H. eapply lsim_mon. *)
+  (*   } *)
 
-    { pfold. eapply pind9_fold. eapply lsim_tidL. split; ss.
-      destruct LSIM0 as [LSIM0 IND]. hexploit IH; eauto. i. punfold H. eapply lsim_mon.
-    }
+  (*   { pfold. eapply pind9_fold. eapply lsim_tidL. split; ss. *)
+  (*     destruct LSIM0 as [LSIM0 IND]. hexploit IH; eauto. i. punfold H. eapply lsim_mon. *)
+  (*   } *)
 
-    { pfold. eapply pind9_fold. eapply lsim_UB. }
+  (*   { pfold. eapply pind9_fold. eapply lsim_UB. } *)
 
-    { des. pfold. eapply pind9_fold. eapply lsim_fairL. esplits; eauto. split; ss.
-      destruct LSIM as [LSIM IND]. hexploit IH; eauto. i. punfold H. eapply lsim_mon.
-    }
+  (*   { des. pfold. eapply pind9_fold. eapply lsim_fairL. esplits; eauto. split; ss. *)
+  (*     destruct LSIM as [LSIM IND]. hexploit IH; eauto. i. punfold H. eapply lsim_mon. *)
+  (*   } *)
 
-    { destruct LSIM0 as [LSIM0 IND]. clear LSIM0.
-      pfold. eapply pind9_fold. eapply lsim_tauR. split; ss.
-      hexploit IH. eauto. all: eauto. i. punfold H. eapply lsim_mon.
-    }
+  (*   { destruct LSIM0 as [LSIM0 IND]. clear LSIM0. *)
+  (*     pfold. eapply pind9_fold. eapply lsim_tauR. split; ss. *)
+  (*     hexploit IH. eauto. all: eauto. i. punfold H. eapply lsim_mon. *)
+  (*   } *)
 
-    { pfold. eapply pind9_fold. eapply lsim_chooseR. i. split; ss. specialize (LSIM0 x).
-      destruct LSIM0 as [LSIM0 IND]. hexploit IH; eauto. i. punfold H. eapply lsim_mon.
-    }
+  (*   { pfold. eapply pind9_fold. eapply lsim_chooseR. i. split; ss. specialize (LSIM0 x). *)
+  (*     destruct LSIM0 as [LSIM0 IND]. hexploit IH; eauto. i. punfold H. eapply lsim_mon. *)
+  (*   } *)
 
-    { pfold. eapply pind9_fold. eapply lsim_putR. split; ss.
-      destruct LSIM0 as [LSIM0 IND]. hexploit IH; eauto. i. punfold H. eapply lsim_mon.
-    }
+  (*   { pfold. eapply pind9_fold. eapply lsim_putR. split; ss. *)
+  (*     destruct LSIM0 as [LSIM0 IND]. hexploit IH; eauto. i. punfold H. eapply lsim_mon. *)
+  (*   } *)
 
-    { pfold. eapply pind9_fold. eapply lsim_getR. split; ss.
-      destruct LSIM0 as [LSIM0 IND]. hexploit IH; eauto. i. punfold H. eapply lsim_mon.
-    }
+  (*   { pfold. eapply pind9_fold. eapply lsim_getR. split; ss. *)
+  (*     destruct LSIM0 as [LSIM0 IND]. hexploit IH; eauto. i. punfold H. eapply lsim_mon. *)
+  (*   } *)
 
-    { pfold. eapply pind9_fold. eapply lsim_tidR. split; ss.
-      destruct LSIM0 as [LSIM0 IND]. hexploit IH; eauto. i. punfold H. eapply lsim_mon.
-    }
+  (*   { pfold. eapply pind9_fold. eapply lsim_tidR. split; ss. *)
+  (*     destruct LSIM0 as [LSIM0 IND]. hexploit IH; eauto. i. punfold H. eapply lsim_mon. *)
+  (*   } *)
 
-    { pfold. eapply pind9_fold. eapply lsim_fairR. i. split; ss. specialize (LSIM0 _ FAIR).
-      des. destruct LSIM0 as [LSIM0 IND]. hexploit IH; eauto. i. punfold H. eapply lsim_mon.
-    }
+  (*   { pfold. eapply pind9_fold. eapply lsim_fairR. i. split; ss. specialize (LSIM0 _ FAIR). *)
+  (*     des. destruct LSIM0 as [LSIM0 IND]. hexploit IH; eauto. i. punfold H. eapply lsim_mon. *)
+  (*   } *)
 
-    { pfold. eapply pind9_fold. eapply lsim_observe. i. eapply upaco9_mon_bot; eauto. }
+  (*   { pfold. eapply pind9_fold. eapply lsim_observe. i. eapply upaco9_mon_bot; eauto. } *)
 
-    { pfold. eapply pind9_fold. eapply lsim_yieldR; eauto. i.
-      hexploit LSIM0; eauto. clear LSIM0. intros LSIM0. des. esplits; eauto.
-      eapply upaco9_mon_bot; eauto.
-    }
+  (*   { pfold. eapply pind9_fold. eapply lsim_yieldR; eauto. i. *)
+  (*     hexploit LSIM0; eauto. clear LSIM0. intros LSIM0. des. esplits; eauto. *)
+  (*     eapply upaco9_mon_bot; eauto. *)
+  (*   } *)
 
-    { des. pfold. eapply pind9_fold. eapply lsim_yieldL. esplits; eauto. split; ss.
-      destruct LSIM as [LSIM IND]. hexploit IH; eauto. i. punfold H. eapply lsim_mon.
-    }
+  (*   { des. pfold. eapply pind9_fold. eapply lsim_yieldL. esplits; eauto. split; ss. *)
+  (*     destruct LSIM as [LSIM IND]. hexploit IH; eauto. i. punfold H. eapply lsim_mon. *)
+  (*   } *)
 
-    { pclearbot. eapply paco9_mon_bot. eapply lsim_reset_prog. eauto. all: ss. }
+  (*   { pfold. eapply pind9_fold. eapply lsim_progress. pclearbot. eapply paco9_mon_bot. eapply lsim_reset_prog. eauto. all: ss. } *)
 
-  Qed.
+  (* Qed. *)
 
   Definition local_RR {R0 R1} (RR: R0 -> R1 -> Prop) tid:
-    R0 -> R1 -> URA.car -> wf_stt.(T) -> shared_rel :=
-    fun (r_src: R0) (r_tgt: R1) (r_ctx: URA.car) (o: wf_stt.(T)) '(ths2, im_src1, im_tgt1, st_src1, st_tgt1, r_shared1) =>
-      (exists ths3 r_own o0 r_shared2,
+    R0 -> R1 -> URA.car -> shared_rel :=
+    fun (r_src: R0) (r_tgt: R1) (r_ctx: URA.car) '(ths2, im_src1, im_tgt1, st_src1, st_tgt1, r_shared1) =>
+      (exists ths3 r_own r_shared2,
           (<<THS: NatMap.remove tid ths2 = ths3>>) /\
             (<<VALID: URA.wf (r_shared2 ⋅ r_own ⋅ r_ctx)>>) /\
             (<<INV: I (ths3, im_src1, im_tgt1, st_src1, st_tgt1, r_shared2)>>) /\
-            (<<STT: wf_stt.(lt) o0 o>>) /\
             (<<RET: RR r_src r_tgt>>)).
 
-  Definition embed_lrr {R0 R1} (LRR: R0 -> R1 -> URA.car -> shared_rel):
-    R0 -> R1 -> URA.car -> wf_stt.(T) -> shared_rel :=
-    fun (r_src: R0) (r_tgt: R1) (r_ctx: URA.car) (o: wf_stt.(T)) shr =>
-      (<<LSIM: LRR r_src r_tgt r_ctx shr>>) /\ (<<STT: exists o0, wf_stt.(lt) o0 o>>).
+  (* Definition local_RR {R0 R1} (RR: R0 -> R1 -> Prop) tid: *)
+  (*   R0 -> R1 -> URA.car -> wf_stt.(T) -> shared_rel := *)
+  (*   fun (r_src: R0) (r_tgt: R1) (r_ctx: URA.car) (o: wf_stt.(T)) '(ths2, im_src1, im_tgt1, st_src1, st_tgt1, r_shared1) => *)
+  (*     (exists ths3 r_own o0 r_shared2, *)
+  (*         (<<THS: NatMap.remove tid ths2 = ths3>>) /\ *)
+  (*           (<<VALID: URA.wf (r_shared2 ⋅ r_own ⋅ r_ctx)>>) /\ *)
+  (*           (<<INV: I (ths3, im_src1, im_tgt1, st_src1, st_tgt1, r_shared2)>>) /\ *)
+  (*           (<<STT: wf_stt.(lt) o0 o>>) /\ *)
+  (*           (<<RET: RR r_src r_tgt>>)). *)
+
+  (* Definition embed_lrr {R0 R1} (LRR: R0 -> R1 -> URA.car -> shared_rel): *)
+  (*   R0 -> R1 -> URA.car -> wf_stt.(T) -> shared_rel := *)
+  (*   fun (r_src: R0) (r_tgt: R1) (r_ctx: URA.car) (o: wf_stt.(T)) shr => *)
+  (*     (<<LSIM: LRR r_src r_tgt r_ctx shr>>) /\ (<<STT: exists o0, wf_stt.(lt) o0 o>>). *)
 
   Definition local_sim {R0 R1} (RR: R0 -> R1 -> Prop) src tgt :=
     forall ths0 im_src0 im_tgt0 st_src0 st_tgt0 r_shared0 r_ctx0
@@ -488,16 +506,16 @@ Section PRIMIVIESIM.
                              (ths, im_src2, im_tgt2, st_src, st_tgt, r_shared2)
                              >>)).
 
-  Definition shared_rel_wf: Prop :=
-    forall ths im_src0 im_tgt0 st_src st_tgt r_shared0 r_ctx
-           (INV: I (ths, im_src0, im_tgt0, st_src, st_tgt, r_shared0))
-           (VALID: URA.wf (r_shared0 ⋅ r_ctx)),
-    forall im_tgt1
-           (TGT: fair_update im_tgt0 im_tgt1 (sum_fmap_l (tids_fmap_all ths))),
-    exists im_src1 r_shared1,
-      (<<SRC: fair_update im_src0 im_src1 (sum_fmap_l (tids_fmap_all ths))>>) /\
-        (<<INV: I (ths, im_src1, im_tgt1, st_src, st_tgt, r_shared1)>>) /\
-        (<<VALID: URA.wf (r_shared1 ⋅ r_ctx)>>).
+  (* Definition shared_rel_wf: Prop := *)
+  (*   forall ths im_src0 im_tgt0 st_src st_tgt r_shared0 r_ctx *)
+  (*          (INV: I (ths, im_src0, im_tgt0, st_src, st_tgt, r_shared0)) *)
+  (*          (VALID: URA.wf (r_shared0 ⋅ r_ctx)), *)
+  (*   forall im_tgt1 *)
+  (*          (TGT: fair_update im_tgt0 im_tgt1 (sum_fmap_l (tids_fmap_all ths))), *)
+  (*   exists im_src1 r_shared1, *)
+  (*     (<<SRC: fair_update im_src0 im_src1 (sum_fmap_l (tids_fmap_all ths))>>) /\ *)
+  (*       (<<INV: I (ths, im_src1, im_tgt1, st_src, st_tgt, r_shared1)>>) /\ *)
+  (*       (<<VALID: URA.wf (r_shared1 ⋅ r_ctx)>>). *)
 
 End PRIMIVIESIM.
 #[export] Hint Constructors __lsim: core.
