src/ModSimNoSync.v
@@ -450,232 +450,232 @@ Section PRIMIVIESIM.
   Local Hint Resolve _lsim_mon: paco.
   Local Hint Resolve lsim_mon: paco.
 
-  Lemma lsim_ind
-        tid
-        (P: forall R0 R1 (RR: R0 -> R1 -> URA.car -> shared_rel), bool -> bool -> URA.car -> (itree srcE R0) -> (itree tgtE R1) -> shared_rel)
-  (RET: forall R0 R1 (RR: R0 -> R1 -> URA.car -> shared_rel)
-      f_src f_tgt r_ctx
-      ths im_src im_tgt st_src st_tgt r_shared
-      r_src r_tgt
-      (LSIM: RR r_src r_tgt r_ctx (ths, im_src, im_tgt, st_src, st_tgt, r_shared)),
-    P R0 R1 RR f_src f_tgt r_ctx (Ret r_src) (Ret r_tgt) (ths, im_src, im_tgt, st_src, st_tgt, r_shared))
-  (TAUL: forall R0 R1 (RR: R0 -> R1 -> URA.car -> shared_rel)
-      f_src f_tgt r_ctx
-      ths im_src im_tgt st_src st_tgt r_shared
-      itr_src itr_tgt
-      (LSIM: lsim tid RR true f_tgt r_ctx itr_src itr_tgt (ths, im_src, im_tgt, st_src, st_tgt, r_shared))
-      (IH: P R0 R1 RR true f_tgt r_ctx itr_src itr_tgt (ths, im_src, im_tgt, st_src, st_tgt, r_shared)),
-    P R0 R1 RR f_src f_tgt r_ctx (Tau itr_src) itr_tgt (ths, im_src, im_tgt, st_src, st_tgt, r_shared))
-  (CHOOSEL: forall R0 R1 (RR: R0 -> R1 -> URA.car -> shared_rel)
-      f_src f_tgt r_ctx
-      ths im_src im_tgt st_src st_tgt r_shared
-      X ktr_src itr_tgt
-      (LSIM: exists x, (<<LSIM: lsim tid RR true f_tgt r_ctx (ktr_src x) itr_tgt (ths, im_src, im_tgt, st_src, st_tgt, r_shared)>>) /\
-      (<<IH: P R0 R1 RR true f_tgt r_ctx (ktr_src x) itr_tgt (ths, im_src, im_tgt, st_src, st_tgt, r_shared)>>)),
-    P R0 R1 RR f_src f_tgt r_ctx (trigger (Choose X) >>= ktr_src) itr_tgt (ths, im_src, im_tgt, st_src, st_tgt, r_shared))
-  (PUTL: forall R0 R1 (RR: R0 -> R1 -> URA.car -> shared_rel)
-      f_src f_tgt r_ctx
-      ths im_src im_tgt st_src st_tgt r_shared
-      st ktr_src itr_tgt
-      (LSIM: lsim tid RR true f_tgt r_ctx (ktr_src tt) itr_tgt (ths, im_src, im_tgt, st, st_tgt, r_shared))
-      (IH: P R0 R1 RR true f_tgt r_ctx (ktr_src tt) itr_tgt (ths, im_src, im_tgt, st, st_tgt, r_shared)),
-    P R0 R1 RR f_src f_tgt r_ctx (trigger (Put st) >>= ktr_src) itr_tgt (ths, im_src, im_tgt, st_src, st_tgt, r_shared))
-  (GETL: forall R0 R1 (RR: R0 -> R1 -> URA.car -> shared_rel)
-      f_src f_tgt r_ctx
-      ths im_src im_tgt st_src st_tgt r_shared
-      ktr_src itr_tgt
-      (LSIM: lsim tid RR true f_tgt r_ctx (ktr_src st_src) itr_tgt (ths, im_src, im_tgt, st_src, st_tgt, r_shared))
-      (IH: P R0 R1 RR true f_tgt r_ctx (ktr_src st_src) itr_tgt (ths, im_src, im_tgt, st_src, st_tgt, r_shared)),
-    P R0 R1 RR f_src f_tgt r_ctx (trigger (@Get _) >>= ktr_src) itr_tgt (ths, im_src, im_tgt, st_src, st_tgt, r_shared))
-  (TIDL: forall R0 R1 (RR: R0 -> R1 -> URA.car -> shared_rel)
-      f_src f_tgt r_ctx
-      ths im_src im_tgt st_src st_tgt r_shared
-      ktr_src itr_tgt
-      (LSIM: lsim tid RR true f_tgt r_ctx (ktr_src tid) itr_tgt (ths, im_src, im_tgt, st_src, st_tgt, r_shared))
-      (IH: P R0 R1 RR true f_tgt r_ctx (ktr_src tid) itr_tgt (ths, im_src, im_tgt, st_src, st_tgt, r_shared)),
-    P R0 R1 RR f_src f_tgt r_ctx (trigger (GetTid) >>= ktr_src) itr_tgt (ths, im_src, im_tgt, st_src, st_tgt, r_shared))
-  (UB: forall R0 R1 (RR: R0 -> R1 -> URA.car -> shared_rel)
-      f_src f_tgt r_ctx
-      ths im_src im_tgt st_src st_tgt r_shared
-      ktr_src itr_tgt,
-    P R0 R1 RR f_src f_tgt r_ctx (trigger (Undefined) >>= ktr_src) itr_tgt (ths, im_src, im_tgt, st_src, st_tgt, r_shared))
-  (FAIRL: forall R0 R1 (RR: R0 -> R1 -> URA.car -> shared_rel)
-      f_src f_tgt r_ctx
-      ths im_src0 im_tgt st_src st_tgt r_shared
-      f ktr_src itr_tgt
-      (LSIM: exists im_src1,
-          (<<FAIR: fair_update im_src0 im_src1 (sum_fmap_r f)>>) /\
-            (<<LSIM: lsim tid RR true f_tgt r_ctx (ktr_src tt) itr_tgt (ths, im_src1, im_tgt, st_src, st_tgt, r_shared)>>) /\
-            (<<IH: P R0 R1 RR true f_tgt r_ctx (ktr_src tt) itr_tgt (ths, im_src1, im_tgt, st_src, st_tgt, r_shared)>>)),
-    P R0 R1 RR f_src f_tgt r_ctx (trigger (Fair f) >>= ktr_src) itr_tgt (ths, im_src0, im_tgt, st_src, st_tgt, r_shared))
+  (* Lemma lsim_ind *)
+  (*       tid *)
+  (*       (P: forall R0 R1 (RR: R0 -> R1 -> URA.car -> shared_rel), bool -> bool -> URA.car -> (itree srcE R0) -> (itree tgtE R1) -> shared_rel) *)
+  (* (RET: forall R0 R1 (RR: R0 -> R1 -> URA.car -> shared_rel) *)
+  (*     f_src f_tgt r_ctx *)
+  (*     ths im_src im_tgt st_src st_tgt r_shared *)
+  (*     r_src r_tgt *)
+  (*     (LSIM: RR r_src r_tgt r_ctx (ths, im_src, im_tgt, st_src, st_tgt, r_shared)), *)
+  (*   P R0 R1 RR f_src f_tgt r_ctx (Ret r_src) (Ret r_tgt) (ths, im_src, im_tgt, st_src, st_tgt, r_shared)) *)
+  (* (TAUL: forall R0 R1 (RR: R0 -> R1 -> URA.car -> shared_rel) *)
+  (*     f_src f_tgt r_ctx *)
+  (*     ths im_src im_tgt st_src st_tgt r_shared *)
+  (*     itr_src itr_tgt *)
+  (*     (LSIM: lsim tid RR true f_tgt r_ctx itr_src itr_tgt (ths, im_src, im_tgt, st_src, st_tgt, r_shared)) *)
+  (*     (IH: P R0 R1 RR true f_tgt r_ctx itr_src itr_tgt (ths, im_src, im_tgt, st_src, st_tgt, r_shared)), *)
+  (*   P R0 R1 RR f_src f_tgt r_ctx (Tau itr_src) itr_tgt (ths, im_src, im_tgt, st_src, st_tgt, r_shared)) *)
+  (* (CHOOSEL: forall R0 R1 (RR: R0 -> R1 -> URA.car -> shared_rel) *)
+  (*     f_src f_tgt r_ctx *)
+  (*     ths im_src im_tgt st_src st_tgt r_shared *)
+  (*     X ktr_src itr_tgt *)
+  (*     (LSIM: exists x, (<<LSIM: lsim tid RR true f_tgt r_ctx (ktr_src x) itr_tgt (ths, im_src, im_tgt, st_src, st_tgt, r_shared)>>) /\ *)
+  (*     (<<IH: P R0 R1 RR true f_tgt r_ctx (ktr_src x) itr_tgt (ths, im_src, im_tgt, st_src, st_tgt, r_shared)>>)), *)
+  (*   P R0 R1 RR f_src f_tgt r_ctx (trigger (Choose X) >>= ktr_src) itr_tgt (ths, im_src, im_tgt, st_src, st_tgt, r_shared)) *)
+  (* (PUTL: forall R0 R1 (RR: R0 -> R1 -> URA.car -> shared_rel) *)
+  (*     f_src f_tgt r_ctx *)
+  (*     ths im_src im_tgt st_src st_tgt r_shared *)
+  (*     st ktr_src itr_tgt *)
+  (*     (LSIM: lsim tid RR true f_tgt r_ctx (ktr_src tt) itr_tgt (ths, im_src, im_tgt, st, st_tgt, r_shared)) *)
+  (*     (IH: P R0 R1 RR true f_tgt r_ctx (ktr_src tt) itr_tgt (ths, im_src, im_tgt, st, st_tgt, r_shared)), *)
+  (*   P R0 R1 RR f_src f_tgt r_ctx (trigger (Put st) >>= ktr_src) itr_tgt (ths, im_src, im_tgt, st_src, st_tgt, r_shared)) *)
+  (* (GETL: forall R0 R1 (RR: R0 -> R1 -> URA.car -> shared_rel) *)
+  (*     f_src f_tgt r_ctx *)
+  (*     ths im_src im_tgt st_src st_tgt r_shared *)
+  (*     ktr_src itr_tgt *)
+  (*     (LSIM: lsim tid RR true f_tgt r_ctx (ktr_src st_src) itr_tgt (ths, im_src, im_tgt, st_src, st_tgt, r_shared)) *)
+  (*     (IH: P R0 R1 RR true f_tgt r_ctx (ktr_src st_src) itr_tgt (ths, im_src, im_tgt, st_src, st_tgt, r_shared)), *)
+  (*   P R0 R1 RR f_src f_tgt r_ctx (trigger (@Get _) >>= ktr_src) itr_tgt (ths, im_src, im_tgt, st_src, st_tgt, r_shared)) *)
+  (* (TIDL: forall R0 R1 (RR: R0 -> R1 -> URA.car -> shared_rel) *)
+  (*     f_src f_tgt r_ctx *)
+  (*     ths im_src im_tgt st_src st_tgt r_shared *)
+  (*     ktr_src itr_tgt *)
+  (*     (LSIM: lsim tid RR true f_tgt r_ctx (ktr_src tid) itr_tgt (ths, im_src, im_tgt, st_src, st_tgt, r_shared)) *)
+  (*     (IH: P R0 R1 RR true f_tgt r_ctx (ktr_src tid) itr_tgt (ths, im_src, im_tgt, st_src, st_tgt, r_shared)), *)
+  (*   P R0 R1 RR f_src f_tgt r_ctx (trigger (GetTid) >>= ktr_src) itr_tgt (ths, im_src, im_tgt, st_src, st_tgt, r_shared)) *)
+  (* (UB: forall R0 R1 (RR: R0 -> R1 -> URA.car -> shared_rel) *)
+  (*     f_src f_tgt r_ctx *)
+  (*     ths im_src im_tgt st_src st_tgt r_shared *)
+  (*     ktr_src itr_tgt, *)
+  (*   P R0 R1 RR f_src f_tgt r_ctx (trigger (Undefined) >>= ktr_src) itr_tgt (ths, im_src, im_tgt, st_src, st_tgt, r_shared)) *)
+  (* (FAIRL: forall R0 R1 (RR: R0 -> R1 -> URA.car -> shared_rel) *)
+  (*     f_src f_tgt r_ctx *)
+  (*     ths im_src0 im_tgt st_src st_tgt r_shared *)
+  (*     f ktr_src itr_tgt *)
+  (*     (LSIM: exists im_src1, *)
+  (*         (<<FAIR: fair_update im_src0 im_src1 (sum_fmap_r f)>>) /\ *)
+  (*           (<<LSIM: lsim tid RR true f_tgt r_ctx (ktr_src tt) itr_tgt (ths, im_src1, im_tgt, st_src, st_tgt, r_shared)>>) /\ *)
+  (*           (<<IH: P R0 R1 RR true f_tgt r_ctx (ktr_src tt) itr_tgt (ths, im_src1, im_tgt, st_src, st_tgt, r_shared)>>)), *)
+  (*   P R0 R1 RR f_src f_tgt r_ctx (trigger (Fair f) >>= ktr_src) itr_tgt (ths, im_src0, im_tgt, st_src, st_tgt, r_shared)) *)
 
-  (TAUR: forall R0 R1 (RR: R0 -> R1 -> URA.car -> shared_rel)
-      f_src f_tgt r_ctx
-      ths im_src im_tgt st_src st_tgt r_shared
-      itr_src itr_tgt
-      (LSIM: lsim tid RR f_src true r_ctx itr_src itr_tgt (ths, im_src, im_tgt, st_src, st_tgt, r_shared))
-      (IH: P R0 R1 RR f_src true r_ctx itr_src itr_tgt (ths, im_src, im_tgt, st_src, st_tgt, r_shared)),
-    P R0 R1 RR f_src f_tgt r_ctx itr_src (Tau itr_tgt) (ths, im_src, im_tgt, st_src, st_tgt, r_shared))
-  (CHOOSER: forall R0 R1 (RR: R0 -> R1 -> URA.car -> shared_rel)
-      f_src f_tgt r_ctx
-      ths im_src im_tgt st_src st_tgt r_shared
-      X itr_src ktr_tgt
-      (LSIM: forall x,
-          (<<LSIM: lsim tid RR f_src true r_ctx itr_src (ktr_tgt x) (ths, im_src, im_tgt, st_src, st_tgt, r_shared)>>) /\
-          (<<IH: P R0 R1 RR f_src true r_ctx itr_src (ktr_tgt x) (ths, im_src, im_tgt, st_src, st_tgt, r_shared)>>)),
-    P R0 R1 RR f_src f_tgt r_ctx itr_src (trigger (Choose X) >>= ktr_tgt) (ths, im_src, im_tgt, st_src, st_tgt, r_shared))
-  (PUTR: forall R0 R1 (RR: R0 -> R1 -> URA.car -> shared_rel)
-      f_src f_tgt r_ctx
-      ths im_src im_tgt st_src st_tgt r_shared
-      st itr_src ktr_tgt
-      (LSIM: lsim tid RR f_src true r_ctx itr_src (ktr_tgt tt) (ths, im_src, im_tgt, st_src, st, r_shared))
-      (IH: P R0 R1 RR f_src true r_ctx itr_src (ktr_tgt tt) (ths, im_src, im_tgt, st_src, st, r_shared)),
-    P R0 R1 RR f_src f_tgt r_ctx itr_src (trigger (Put st) >>= ktr_tgt) (ths, im_src, im_tgt, st_src, st_tgt, r_shared))
-  (GETR: forall R0 R1 (RR: R0 -> R1 -> URA.car -> shared_rel)
-      f_src f_tgt r_ctx
-      ths im_src im_tgt st_src st_tgt r_shared
-      itr_src ktr_tgt
-      (LSIM: lsim tid RR f_src true r_ctx itr_src (ktr_tgt st_tgt) (ths, im_src, im_tgt, st_src, st_tgt, r_shared)),
-    P R0 R1 RR f_src f_tgt r_ctx itr_src (trigger (@Get _) >>= ktr_tgt) (ths, im_src, im_tgt, st_src, st_tgt, r_shared))
-  (TIDR: forall R0 R1 (RR: R0 -> R1 -> URA.car -> shared_rel)
-      f_src f_tgt r_ctx
-      ths im_src im_tgt st_src st_tgt r_shared
-      itr_src ktr_tgt
-      (LSIM: lsim tid RR f_src true r_ctx itr_src (ktr_tgt tid) (ths, im_src, im_tgt, st_src, st_tgt, r_shared)),
-    P R0 R1 RR f_src f_tgt r_ctx itr_src (trigger (GetTid) >>= ktr_tgt) (ths, im_src, im_tgt, st_src, st_tgt, r_shared))
-  (FAIRR: forall R0 R1 (RR: R0 -> R1 -> URA.car -> shared_rel)
-      f_src f_tgt r_ctx
-      ths im_src im_tgt0 st_src st_tgt r_shared
-      f itr_src ktr_tgt
-      (LSIM: forall im_tgt1
-                   (FAIR: fair_update im_tgt0 im_tgt1 (sum_fmap_r f)),
-          (<<LSIM: lsim tid RR f_src true r_ctx itr_src (ktr_tgt tt) (ths, im_src, im_tgt1, st_src, st_tgt, r_shared)>>) /\
-          (<<IH: P R0 R1 RR f_src true r_ctx itr_src (ktr_tgt tt) (ths, im_src, im_tgt1, st_src, st_tgt, r_shared)>>)),
-    P R0 R1 RR f_src f_tgt r_ctx itr_src (trigger (Fair f) >>= ktr_tgt) (ths, im_src, im_tgt0, st_src, st_tgt, r_shared))
+  (* (TAUR: forall R0 R1 (RR: R0 -> R1 -> URA.car -> shared_rel) *)
+  (*     f_src f_tgt r_ctx *)
+  (*     ths im_src im_tgt st_src st_tgt r_shared *)
+  (*     itr_src itr_tgt *)
+  (*     (LSIM: lsim tid RR f_src true r_ctx itr_src itr_tgt (ths, im_src, im_tgt, st_src, st_tgt, r_shared)) *)
+  (*     (IH: P R0 R1 RR f_src true r_ctx itr_src itr_tgt (ths, im_src, im_tgt, st_src, st_tgt, r_shared)), *)
+  (*   P R0 R1 RR f_src f_tgt r_ctx itr_src (Tau itr_tgt) (ths, im_src, im_tgt, st_src, st_tgt, r_shared)) *)
+  (* (CHOOSER: forall R0 R1 (RR: R0 -> R1 -> URA.car -> shared_rel) *)
+  (*     f_src f_tgt r_ctx *)
+  (*     ths im_src im_tgt st_src st_tgt r_shared *)
+  (*     X itr_src ktr_tgt *)
+  (*     (LSIM: forall x, *)
+  (*         (<<LSIM: lsim tid RR f_src true r_ctx itr_src (ktr_tgt x) (ths, im_src, im_tgt, st_src, st_tgt, r_shared)>>) /\ *)
+  (*         (<<IH: P R0 R1 RR f_src true r_ctx itr_src (ktr_tgt x) (ths, im_src, im_tgt, st_src, st_tgt, r_shared)>>)), *)
+  (*   P R0 R1 RR f_src f_tgt r_ctx itr_src (trigger (Choose X) >>= ktr_tgt) (ths, im_src, im_tgt, st_src, st_tgt, r_shared)) *)
+  (* (PUTR: forall R0 R1 (RR: R0 -> R1 -> URA.car -> shared_rel) *)
+  (*     f_src f_tgt r_ctx *)
+  (*     ths im_src im_tgt st_src st_tgt r_shared *)
+  (*     st itr_src ktr_tgt *)
+  (*     (LSIM: lsim tid RR f_src true r_ctx itr_src (ktr_tgt tt) (ths, im_src, im_tgt, st_src, st, r_shared)) *)
+  (*     (IH: P R0 R1 RR f_src true r_ctx itr_src (ktr_tgt tt) (ths, im_src, im_tgt, st_src, st, r_shared)), *)
+  (*   P R0 R1 RR f_src f_tgt r_ctx itr_src (trigger (Put st) >>= ktr_tgt) (ths, im_src, im_tgt, st_src, st_tgt, r_shared)) *)
+  (* (GETR: forall R0 R1 (RR: R0 -> R1 -> URA.car -> shared_rel) *)
+  (*     f_src f_tgt r_ctx *)
+  (*     ths im_src im_tgt st_src st_tgt r_shared *)
+  (*     itr_src ktr_tgt *)
+  (*     (LSIM: lsim tid RR f_src true r_ctx itr_src (ktr_tgt st_tgt) (ths, im_src, im_tgt, st_src, st_tgt, r_shared)), *)
+  (*   P R0 R1 RR f_src f_tgt r_ctx itr_src (trigger (@Get _) >>= ktr_tgt) (ths, im_src, im_tgt, st_src, st_tgt, r_shared)) *)
+  (* (TIDR: forall R0 R1 (RR: R0 -> R1 -> URA.car -> shared_rel) *)
+  (*     f_src f_tgt r_ctx *)
+  (*     ths im_src im_tgt st_src st_tgt r_shared *)
+  (*     itr_src ktr_tgt *)
+  (*     (LSIM: lsim tid RR f_src true r_ctx itr_src (ktr_tgt tid) (ths, im_src, im_tgt, st_src, st_tgt, r_shared)), *)
+  (*   P R0 R1 RR f_src f_tgt r_ctx itr_src (trigger (GetTid) >>= ktr_tgt) (ths, im_src, im_tgt, st_src, st_tgt, r_shared)) *)
+  (* (FAIRR: forall R0 R1 (RR: R0 -> R1 -> URA.car -> shared_rel) *)
+  (*     f_src f_tgt r_ctx *)
+  (*     ths im_src im_tgt0 st_src st_tgt r_shared *)
+  (*     f itr_src ktr_tgt *)
+  (*     (LSIM: forall im_tgt1 *)
+  (*                  (FAIR: fair_update im_tgt0 im_tgt1 (sum_fmap_r f)), *)
+  (*         (<<LSIM: lsim tid RR f_src true r_ctx itr_src (ktr_tgt tt) (ths, im_src, im_tgt1, st_src, st_tgt, r_shared)>>) /\ *)
+  (*         (<<IH: P R0 R1 RR f_src true r_ctx itr_src (ktr_tgt tt) (ths, im_src, im_tgt1, st_src, st_tgt, r_shared)>>)), *)
+  (*   P R0 R1 RR f_src f_tgt r_ctx itr_src (trigger (Fair f) >>= ktr_tgt) (ths, im_src, im_tgt0, st_src, st_tgt, r_shared)) *)
 
-  (OBSERVE: forall R0 R1 (RR: R0 -> R1 -> URA.car -> shared_rel)
-      f_src f_tgt r_ctx
-      ths im_src im_tgt st_src st_tgt r_shared
-      fn args ktr_src ktr_tgt
-      (LSIM: forall ret,
-          (<<LSIM: lsim tid RR true true r_ctx (ktr_src ret) (ktr_tgt ret) (ths, im_src, im_tgt, st_src, st_tgt, r_shared)>>) /\
-          (<<IH: P R0 R1 RR true true r_ctx (ktr_src ret) (ktr_tgt ret) (ths, im_src, im_tgt, st_src, st_tgt, r_shared)>>)),
-    P R0 R1 RR f_src f_tgt r_ctx (trigger (Observe fn args) >>= ktr_src) (trigger (Observe fn args) >>= ktr_tgt) (ths, im_src, im_tgt, st_src, st_tgt, r_shared))
+  (* (OBSERVE: forall R0 R1 (RR: R0 -> R1 -> URA.car -> shared_rel) *)
+  (*     f_src f_tgt r_ctx *)
+  (*     ths im_src im_tgt st_src st_tgt r_shared *)
+  (*     fn args ktr_src ktr_tgt *)
+  (*     (LSIM: forall ret, *)
+  (*         (<<LSIM: lsim tid RR true true r_ctx (ktr_src ret) (ktr_tgt ret) (ths, im_src, im_tgt, st_src, st_tgt, r_shared)>>) /\ *)
+  (*         (<<IH: P R0 R1 RR true true r_ctx (ktr_src ret) (ktr_tgt ret) (ths, im_src, im_tgt, st_src, st_tgt, r_shared)>>)), *)
+  (*   P R0 R1 RR f_src f_tgt r_ctx (trigger (Observe fn args) >>= ktr_src) (trigger (Observe fn args) >>= ktr_tgt) (ths, im_src, im_tgt, st_src, st_tgt, r_shared)) *)
 
-  (YIELDR: forall R0 R1 (RR: R0 -> R1 -> URA.car -> shared_rel)
-      f_src f_tgt r_ctx0
-      ths0 im_src0 im_tgt0 st_src0 st_tgt0 r_shared0
-      r_own r_shared
-      ktr_src ktr_tgt
-      (INV: I (ths0, im_src0, im_tgt0, st_src0, st_tgt0, r_shared))
-      (VALID: URA.wf (r_shared ⋅ r_own ⋅ r_ctx0))
-      (LSIM: forall ths1 im_src1 im_tgt1 st_src1 st_tgt1 r_shared1 r_ctx1
-                    (INV: I (ths1, im_src1, im_tgt1, st_src1, st_tgt1, r_shared1))
-                    (VALID: URA.wf (r_shared1 ⋅ r_own ⋅ r_ctx1))
-                    im_tgt2
-                    (TGT: fair_update im_tgt1 im_tgt2 (sum_fmap_l (tids_fmap tid ths1))),
-          (<<LSIM: lsim tid RR f_src true r_ctx1 (trigger (Yield) >>= ktr_src) (ktr_tgt tt) (ths1, im_src1, im_tgt2, st_src1, st_tgt1, r_shared1)>>) /\
-            (<<IH: P R0 R1 RR f_src true r_ctx1 (trigger (Yield) >>= ktr_src) (ktr_tgt tt) (ths1, im_src1, im_tgt2, st_src1, st_tgt1, r_shared1)>>)),
-    P R0 R1 RR f_src f_tgt r_ctx0 (trigger (Yield) >>= ktr_src) (trigger (Yield) >>= ktr_tgt) (ths0, im_src0, im_tgt0, st_src0, st_tgt0, r_shared0))
-  (YIELDL: forall R0 R1 (RR: R0 -> R1 -> URA.car -> shared_rel)
-      f_src f_tgt r_ctx
-      ths im_src0 im_tgt st_src st_tgt r_shared
-      ktr_src itr_tgt
-      (LSIM: exists im_src1,
-          (<<FAIR: fair_update im_src0 im_src1 (sum_fmap_l (tids_fmap tid ths))>>) /\
-            (<<LSIM: lsim tid RR true f_tgt r_ctx (ktr_src tt) itr_tgt (ths, im_src1, im_tgt, st_src, st_tgt, r_shared)>>) /\
-            (<<IH: P R0 R1 RR true f_tgt r_ctx (ktr_src tt) itr_tgt (ths, im_src1, im_tgt, st_src, st_tgt, r_shared)>>)),
-    P R0 R1 RR f_src f_tgt r_ctx (trigger (Yield) >>= ktr_src) itr_tgt (ths, im_src0, im_tgt, st_src, st_tgt, r_shared))
+  (* (YIELDR: forall R0 R1 (RR: R0 -> R1 -> URA.car -> shared_rel) *)
+  (*     f_src f_tgt r_ctx0 *)
+  (*     ths0 im_src0 im_tgt0 st_src0 st_tgt0 r_shared0 *)
+  (*     r_own r_shared *)
+  (*     ktr_src ktr_tgt *)
+  (*     (INV: I (ths0, im_src0, im_tgt0, st_src0, st_tgt0, r_shared)) *)
+  (*     (VALID: URA.wf (r_shared ⋅ r_own ⋅ r_ctx0)) *)
+  (*     (LSIM: forall ths1 im_src1 im_tgt1 st_src1 st_tgt1 r_shared1 r_ctx1 *)
+  (*                   (INV: I (ths1, im_src1, im_tgt1, st_src1, st_tgt1, r_shared1)) *)
+  (*                   (VALID: URA.wf (r_shared1 ⋅ r_own ⋅ r_ctx1)) *)
+  (*                   im_tgt2 *)
+  (*                   (TGT: fair_update im_tgt1 im_tgt2 (sum_fmap_l (tids_fmap tid ths1))), *)
+  (*         (<<LSIM: lsim tid RR f_src true r_ctx1 (trigger (Yield) >>= ktr_src) (ktr_tgt tt) (ths1, im_src1, im_tgt2, st_src1, st_tgt1, r_shared1)>>) /\ *)
+  (*           (<<IH: P R0 R1 RR f_src true r_ctx1 (trigger (Yield) >>= ktr_src) (ktr_tgt tt) (ths1, im_src1, im_tgt2, st_src1, st_tgt1, r_shared1)>>)), *)
+  (*   P R0 R1 RR f_src f_tgt r_ctx0 (trigger (Yield) >>= ktr_src) (trigger (Yield) >>= ktr_tgt) (ths0, im_src0, im_tgt0, st_src0, st_tgt0, r_shared0)) *)
+  (* (YIELDL: forall R0 R1 (RR: R0 -> R1 -> URA.car -> shared_rel) *)
+  (*     f_src f_tgt r_ctx *)
+  (*     ths im_src0 im_tgt st_src st_tgt r_shared *)
+  (*     ktr_src itr_tgt *)
+  (*     (LSIM: exists im_src1, *)
+  (*         (<<FAIR: fair_update im_src0 im_src1 (sum_fmap_l (tids_fmap tid ths))>>) /\ *)
+  (*           (<<LSIM: lsim tid RR true f_tgt r_ctx (ktr_src tt) itr_tgt (ths, im_src1, im_tgt, st_src, st_tgt, r_shared)>>) /\ *)
+  (*           (<<IH: P R0 R1 RR true f_tgt r_ctx (ktr_src tt) itr_tgt (ths, im_src1, im_tgt, st_src, st_tgt, r_shared)>>)), *)
+  (*   P R0 R1 RR f_src f_tgt r_ctx (trigger (Yield) >>= ktr_src) itr_tgt (ths, im_src0, im_tgt, st_src, st_tgt, r_shared)) *)
 
-  (PROG: forall R0 R1 (RR: R0 -> R1 -> URA.car -> shared_rel)
-      r_ctx
-      ths im_src im_tgt st_src st_tgt r_shared
-      itr_src itr_tgt
-      (LSIM: lsim tid RR false false r_ctx itr_src itr_tgt (ths, im_src, im_tgt, st_src, st_tgt, r_shared)),
-      P R0 R1 RR true true r_ctx itr_src itr_tgt (ths, im_src, im_tgt, st_src, st_tgt, r_shared))
-    :
-    forall R0 R1 (RR: R0 -> R1 -> URA.car -> shared_rel) f_src f_tgt r_ctx ths im_src im_tgt st_src st_tgt r_shared itr_src itr_tgt
-      (LSIM: lsim tid RR f_src f_tgt r_ctx itr_src itr_tgt (ths, im_src, im_tgt, st_src, st_tgt, r_shared)),
-      P R0 R1 RR f_src f_tgt r_ctx itr_src itr_tgt (ths, im_src, im_tgt, st_src, st_tgt, r_shared).
-  Proof.
-    i. match goal with | LSIM: lsim tid RR _ _ _ _ _ ?_shr |- _ => remember _shr as shr end.
-    move LSIM before PROG. revert_until LSIM.
-    punfold LSIM.
-    pattern R0, R1, RR, f_src, f_tgt, r_ctx, itr_src, itr_tgt, shr.
-    revert R0 R1 RR f_src f_tgt r_ctx itr_src itr_tgt shr LSIM. apply pind9_acc.
-    intros rr DEC IH. clear DEC. intros R0 R1 RR f_src f_tgt r_ctx itr_src itr_tgt shr LSIM.
-    i. clarify.
-    eapply pind9_unfold in LSIM.
-    2:{ eapply _lsim_mon. }
-    inv LSIM.
+  (* (PROG: forall R0 R1 (RR: R0 -> R1 -> URA.car -> shared_rel) *)
+  (*     r_ctx *)
+  (*     ths im_src im_tgt st_src st_tgt r_shared *)
+  (*     itr_src itr_tgt *)
+  (*     (LSIM: lsim tid RR false false r_ctx itr_src itr_tgt (ths, im_src, im_tgt, st_src, st_tgt, r_shared)), *)
+  (*     P R0 R1 RR true true r_ctx itr_src itr_tgt (ths, im_src, im_tgt, st_src, st_tgt, r_shared)) *)
+  (*   : *)
+  (*   forall R0 R1 (RR: R0 -> R1 -> URA.car -> shared_rel) f_src f_tgt r_ctx ths im_src im_tgt st_src st_tgt r_shared itr_src itr_tgt *)
+  (*     (LSIM: lsim tid RR f_src f_tgt r_ctx itr_src itr_tgt (ths, im_src, im_tgt, st_src, st_tgt, r_shared)), *)
+  (*     P R0 R1 RR f_src f_tgt r_ctx itr_src itr_tgt (ths, im_src, im_tgt, st_src, st_tgt, r_shared). *)
+  (* Proof. *)
+  (*   i. match goal with | LSIM: lsim tid RR _ _ _ _ _ ?_shr |- _ => remember _shr as shr end. *)
+  (*   move LSIM before PROG. revert_until LSIM. *)
+  (*   punfold LSIM. *)
+  (*   pattern R0, R1, RR, f_src, f_tgt, r_ctx, itr_src, itr_tgt, shr. *)
+  (*   revert R0 R1 RR f_src f_tgt r_ctx itr_src itr_tgt shr LSIM. apply pind9_acc. *)
+  (*   intros rr DEC IH. clear DEC. intros R0 R1 RR f_src f_tgt r_ctx itr_src itr_tgt shr LSIM. *)
+  (*   i. clarify. *)
+  (*   eapply pind9_unfold in LSIM. *)
+  (*   2:{ eapply _lsim_mon. } *)
+  (*   inv LSIM. *)
 
-    { eapply RET; eauto. }
+  (*   { eapply RET; eauto. } *)
 
-    { destruct LSIM0 as [LSIM IND]. eapply TAUL; eauto.
-      pfold. eapply pind9_mon_top; eauto.
-    }
+  (*   { destruct LSIM0 as [LSIM IND]. eapply TAUL; eauto. *)
+  (*     pfold. eapply pind9_mon_top; eauto. *)
+  (*   } *)
 
-    { des. eapply CHOOSEL; eauto. exists x.
-      destruct LSIM0 as [LSIM IND]. splits; eauto. pfold. eapply pind9_mon_top; eauto.
-    }
+  (*   { des. eapply CHOOSEL; eauto. exists x. *)
+  (*     destruct LSIM0 as [LSIM IND]. splits; eauto. pfold. eapply pind9_mon_top; eauto. *)
+  (*   } *)
 
-    { destruct LSIM0 as [LSIM IND]. eapply PUTL; eauto.
-      pfold. eapply pind9_mon_top; eauto.
-    }
+  (*   { destruct LSIM0 as [LSIM IND]. eapply PUTL; eauto. *)
+  (*     pfold. eapply pind9_mon_top; eauto. *)
+  (*   } *)
 
-    { destruct LSIM0 as [LSIM IND]. eapply GETL; eauto.
-      pfold. eapply pind9_mon_top; eauto.
-    }
+  (*   { destruct LSIM0 as [LSIM IND]. eapply GETL; eauto. *)
+  (*     pfold. eapply pind9_mon_top; eauto. *)
+  (*   } *)
 
-    { destruct LSIM0 as [LSIM IND]. eapply TIDL; eauto.
-      pfold. eapply pind9_mon_top; eauto.
-    }
+  (*   { destruct LSIM0 as [LSIM IND]. eapply TIDL; eauto. *)
+  (*     pfold. eapply pind9_mon_top; eauto. *)
+  (*   } *)
 
-    { eapply UB; eauto. }
+  (*   { eapply UB; eauto. } *)
 
-    { des. destruct LSIM as [LSIM IND].
-      eapply FAIRL. esplits; eauto. pfold. eapply pind9_mon_top; eauto.
-    }
+  (*   { des. destruct LSIM as [LSIM IND]. *)
+  (*     eapply FAIRL. esplits; eauto. pfold. eapply pind9_mon_top; eauto. *)
+  (*   } *)
 
-    { destruct LSIM0 as [LSIM IND]. eapply TAUR; eauto.
-      pfold. eapply pind9_mon_top; eauto.
-    }
+  (*   { destruct LSIM0 as [LSIM IND]. eapply TAUR; eauto. *)
+  (*     pfold. eapply pind9_mon_top; eauto. *)
+  (*   } *)
 
-    { eapply CHOOSER; eauto. i. specialize (LSIM0 x). destruct LSIM0 as [LSIM IND]. splits; eauto.
-      pfold. eapply pind9_mon_top; eauto.
-    }
+  (*   { eapply CHOOSER; eauto. i. specialize (LSIM0 x). destruct LSIM0 as [LSIM IND]. splits; eauto. *)
+  (*     pfold. eapply pind9_mon_top; eauto. *)
+  (*   } *)
 
-    { destruct LSIM0 as [LSIM IND]. eapply PUTR; eauto.
-      pfold. eapply pind9_mon_top; eauto.
-    }
+  (*   { destruct LSIM0 as [LSIM IND]. eapply PUTR; eauto. *)
+  (*     pfold. eapply pind9_mon_top; eauto. *)
+  (*   } *)
 
-    { destruct LSIM0 as [LSIM IND]. eapply GETR; eauto.
-      pfold. eapply pind9_mon_top; eauto.
-    }
+  (*   { destruct LSIM0 as [LSIM IND]. eapply GETR; eauto. *)
+  (*     pfold. eapply pind9_mon_top; eauto. *)
+  (*   } *)
 
-    { destruct LSIM0 as [LSIM IND]. eapply TIDR; eauto.
-      pfold. eapply pind9_mon_top; eauto.
-    }
+  (*   { destruct LSIM0 as [LSIM IND]. eapply TIDR; eauto. *)
+  (*     pfold. eapply pind9_mon_top; eauto. *)
+  (*   } *)
 
-    { eapply FAIRR; eauto. i. specialize (LSIM0 _ FAIR). destruct LSIM0 as [LSIM IND]. splits; eauto.
-      pfold. eapply pind9_mon_top; eauto.
-    }
+  (*   { eapply FAIRR; eauto. i. specialize (LSIM0 _ FAIR). destruct LSIM0 as [LSIM IND]. splits; eauto. *)
+  (*     pfold. eapply pind9_mon_top; eauto. *)
+  (*   } *)
 
-    { eapply OBSERVE. i. specialize (LSIM0 ret). destruct LSIM0 as [LSIM IND]. splits; eauto.
-      pfold. eapply pind9_mon_top; eauto.
-    }
+  (*   { eapply OBSERVE. i. specialize (LSIM0 ret). destruct LSIM0 as [LSIM IND]. splits; eauto. *)
+  (*     pfold. eapply pind9_mon_top; eauto. *)
+  (*   } *)
 
-    { eapply YIELDR; eauto. i. hexploit LSIM0; clear LSIM0. eapply INV0. eapply VALID0. all: eauto.
-      intros [LSIM IND]. splits; eauto. pfold. eapply pind9_mon_top; eauto.
-    }
+  (*   { eapply YIELDR; eauto. i. hexploit LSIM0; clear LSIM0. eapply INV0. eapply VALID0. all: eauto. *)
+  (*     intros [LSIM IND]. splits; eauto. pfold. eapply pind9_mon_top; eauto. *)
+  (*   } *)
 
-    { des. destruct LSIM as [LSIM IND]. eapply YIELDL; eauto. esplits; eauto.
-      pfold. eapply pind9_mon_top; eauto.
-    }
+  (*   { des. destruct LSIM as [LSIM IND]. eapply YIELDL; eauto. esplits; eauto. *)
+  (*     pfold. eapply pind9_mon_top; eauto. *)
+  (*   } *)
 
-    { pclearbot. eapply PROG; eauto. }
+  (*   { pclearbot. eapply PROG; eauto. } *)
 
-  Qed.
+  (* Qed. *)
 
   Definition local_RR {R0 R1} (RR: R0 -> R1 -> Prop) tid:
     R0 -> R1 -> URA.car -> shared_rel :=
@@ -711,16 +711,16 @@ Section PRIMIVIESIM.
                     (ths, im_src2, im_tgt2, st_src, st_tgt, r_shared2)
                     >>)).
 
-  Definition shared_rel_wf: Prop :=
-    forall ths im_src0 im_tgt0 st_src st_tgt r_shared0 r_ctx
-           (INV: I (ths, im_src0, im_tgt0, st_src, st_tgt, r_shared0))
-           (VALID: URA.wf (r_shared0 ⋅ r_ctx)),
-    forall im_tgt1
-           (TGT: fair_update im_tgt0 im_tgt1 (sum_fmap_l (tids_fmap_all ths))),
-    exists im_src1 r_shared1,
-      (<<SRC: fair_update im_src0 im_src1 (sum_fmap_l (tids_fmap_all ths))>>) /\
-        (<<INV: I (ths, im_src1, im_tgt1, st_src, st_tgt, r_shared1)>>) /\
-        (<<VALID: URA.wf (r_shared1 ⋅ r_ctx)>>).
+  (* Definition shared_rel_wf: Prop := *)
+  (*   forall ths im_src0 im_tgt0 st_src st_tgt r_shared0 r_ctx *)
+  (*          (INV: I (ths, im_src0, im_tgt0, st_src, st_tgt, r_shared0)) *)
+  (*          (VALID: URA.wf (r_shared0 ⋅ r_ctx)), *)
+  (*   forall im_tgt1 *)
+  (*          (TGT: fair_update im_tgt0 im_tgt1 (sum_fmap_l (tids_fmap_all ths))), *)
+  (*   exists im_src1 r_shared1, *)
+  (*     (<<SRC: fair_update im_src0 im_src1 (sum_fmap_l (tids_fmap_all ths))>>) /\ *)
+  (*       (<<INV: I (ths, im_src1, im_tgt1, st_src, st_tgt, r_shared1)>>) /\ *)
+  (*       (<<VALID: URA.wf (r_shared1 ⋅ r_ctx)>>). *)
 
 End PRIMIVIESIM.
 #[export] Hint Constructors __lsim: core.
