src/NoSync2Stutter.v
@@ -45,38 +45,38 @@ Section PROOF.
 
   Variable I: shared_rel.
 
-  Lemma embed_lrr_iff
-        wf_stt
-        R0 R1 (RR: R0 -> R1 -> Prop) tid
-        r0 r1 r_ctx o
-        (shr: shared)
-    :
-    ModSimStutter.local_RR wf_stt I RR tid r0 r1 r_ctx o shr <->
-      embed_lrr wf_stt (ModSimNoSync.local_RR I RR tid) r0 r1 r_ctx o shr.
-  Proof.
-    unfold embed_lrr, ModSimStutter.local_RR, ModSimNoSync.local_RR. des_ifs. split; i; des.
-    - esplits; eauto.
-    - esplits; eauto.
-  Qed.
+  (* Lemma embed_lrr_iff *)
+  (*       wf_stt *)
+  (*       R0 R1 (RR: R0 -> R1 -> Prop) tid *)
+  (*       r0 r1 r_ctx o *)
+  (*       (shr: shared) *)
+  (*   : *)
+  (*   ModSimStutter.local_RR wf_stt I RR tid r0 r1 r_ctx o shr <-> *)
+  (*     embed_lrr wf_stt (ModSimNoSync.local_RR I RR tid) r0 r1 r_ctx o shr. *)
+  (* Proof. *)
+  (*   unfold embed_lrr, ModSimStutter.local_RR, ModSimNoSync.local_RR. des_ifs. split; i; des. *)
+  (*   - esplits; eauto. *)
+  (*   - esplits; eauto. *)
+  (* Qed. *)
 
-  Lemma stutter_lrr_ord_weak
+  Lemma stutter_ord_weak
           wf_stt tid
-          R0 R1 (LRR1 LRR2: R0 -> R1 -> URA.car -> wf_stt.(T) -> shared_rel)
-          (IMPL: forall r0 r1 m o0 o1 shr (LE: wf_stt.(le) o0 o1),
-              LRR1 r0 r1 m o0 shr -> LRR2 r0 r1 m o1 shr)
+          R0 R1 (LRR: R0 -> R1 -> URA.car -> shared_rel)
+          (* (IMPL: forall r0 r1 m o0 o1 shr (LE: wf_stt.(le) o0 o1), *)
+          (*     LRR1 r0 r1 m o0 shr -> LRR2 r0 r1 m o1 shr) *)
           ps pt r_ctx src tgt (shr: shared) o0 o1
-          (LE: wf_stt.(le) o0 o1)
-          (LSIM: ModSimStutter.lsim wf_stt I tid LRR1 ps pt r_ctx (o0, src) tgt shr)
+          (LT: wf_stt.(lt) o0 o1)
+          (LSIM: ModSimStutter.lsim wf_stt I tid LRR ps pt r_ctx (o0, src) tgt shr)
     :
-    ModSimStutter.lsim wf_stt I tid LRR2 ps pt r_ctx (o1, src) tgt shr.
+    ModSimStutter.lsim wf_stt I tid LRR ps pt r_ctx (o1, src) tgt shr.
   Proof.
     revert_until tid. pcofix CIH; i.
     remember (o0, src) as osrc.
     move LSIM before CIH. revert_until LSIM.
     punfold LSIM.
-    pattern R0, R1, LRR1, ps, pt, r_ctx, osrc, tgt, shr.
-    revert R0 R1 LRR1 ps pt r_ctx osrc tgt shr LSIM. apply pind9_acc.
-    intros rr DEC IH. clear DEC. intros R0 R1 LRR1 ps pt r_ctx osrc tgt shr LSIM.
+    pattern R0, R1, LRR, ps, pt, r_ctx, osrc, tgt, shr.
+    revert R0 R1 LRR ps pt r_ctx osrc tgt shr LSIM. apply pind9_acc.
+    intros rr DEC IH. clear DEC. intros R0 R1 LRR ps pt r_ctx osrc tgt shr LSIM.
     i; clarify.
     eapply pind9_unfold in LSIM.
     2:{ eapply ModSimStutter._lsim_mon. }
@@ -129,175 +129,25 @@ Section PROOF.
       right. eapply CIH; eauto.
     }
 
-    { unfold le in LE; des; clarify.
-      - pfold. eapply pind9_fold. eapply ModSimStutter.lsim_yieldR; eauto.
-        i. hexploit LSIM0; clear LSIM0; eauto; intro LSIM. des. esplits; eauto.
-        pclearbot. right. eapply CIH; eauto. left; auto.
-      - rename LE into LT.
-        pfold. eapply pind9_fold. eapply ModSimStutter.lsim_yieldR; eauto.
-        i. hexploit LSIM0; clear LSIM0; eauto; intro LSIM. des. esplits; eauto.
-        pclearbot. right. eapply CIH; eauto. right; auto.
+    { pfold. eapply pind9_fold. eapply ModSimStutter.lsim_yieldR; eauto.
+      i. hexploit LSIM0; clear LSIM0; eauto; intro LSIM. des. esplits; eauto.
+      pclearbot. right. eapply CIH; eauto.
     }
 
     { pfold. eapply pind9_fold. eapply ModSimStutter.lsim_yieldL; eauto.
       des. esplits; eauto. destruct LSIM as [LSIM IND].
-      split; ss. eapply IH in IND. punfold IND. eauto. 2: eauto. left; eauto.
+      split; ss. eapply pind9_mon_gen. eapply LSIM.
+      - i. eapply __lsim_mon. 2: eapply PR. i. eapply upaco9_mon_bot; eauto.
+      - ss.
     }
 
-    { pfold. eapply pind9_fold. eapply ModSimStutter.lsim_progress. right.
-      eapply CIH; eauto. pclearbot. auto.
-    }
+    { pfold. eapply pind9_fold. eapply ModSimStutter.lsim_progress. auto. }
 
   Qed.
 
 
-  Let RR_rel R0 R1 := R0 -> R1 -> URA.car -> shared_rel.
   Let A R0 R1 := (bool * bool * URA.car * (itree srcE R0) * (itree tgtE R1) * shared)%type.
   Let wf_stt {R0 R1} := (@ord_tree_WF (A R0 R1)).
-
-  (* Lemma nosync_implies_stutter_prog *)
-  (*       tid *)
-  (*       R0 R1 (LRR: R0 -> R1 -> URA.car -> shared_rel) *)
-  (*       ps pt r_ctx src tgt *)
-  (*       (shr: shared) *)
-  (*       (PROG: ps = true) *)
-  (*       (LSIM: ModSimNoSync.lsim I tid LRR ps pt r_ctx src tgt shr) *)
-  (*   : *)
-  (*   exists (o: (@wf_stt R0 R1).(T)), *)
-  (*     ModSimStutter.lsim wf_stt I tid (embed_lrr wf_stt LRR) ps pt r_ctx (o, src) tgt shr. *)
-  (* Proof. *)
-  (*   move LSIM before LRR. revert_until LSIM. *)
-  (*   punfold LSIM. *)
-  (*   pattern R0, R1, LRR, ps, pt, r_ctx, src, tgt, shr. *)
-  (*   revert R0 R1 LRR ps pt r_ctx src tgt shr LSIM. apply pind9_acc. *)
-  (*   intros rr DEC IH. clear DEC. intros R0 R1 LRR ps pt r_ctx src tgt shr LSIM. *)
-  (*   intros PROG. clarify. *)
-  (*   eapply pind9_unfold in LSIM. *)
-  (*   2:{ eapply ModSimNoSync._lsim_mon. } *)
-  (*   inv LSIM. *)
-
-  (*   { remember (fun _: (A R0 R1) => @ord_tree_base (A R0 R1)) as ao. exists (ord_tree_cons ao). *)
-  (*     pfold. eapply pind9_fold. econs 1; eauto. *)
-  (*     unfold embed_lrr. splits; auto. ss. *)
-  (*     exists (ao (true, pt, r_ctx, Ret r_src, Ret r_tgt, (ths, im_src, im_tgt, st_src, st_tgt, r_shared))). *)
-  (*     eapply ord_tree_lt_intro. *)
-  (*   } *)
-
-  (*   { destruct LSIM0 as [LSIM IND]. eapply IH in IND. des. exists o. *)
-  (*     pfold. eapply pind9_fold. econs 2; eauto. *)
-  (*     split; ss. punfold IND. auto. *)
-  (*   } *)
-  (*   { des. destruct LSIM0 as [LSIM IND]. eapply IH in IND. des. exists o. *)
-  (*     pfold. eapply pind9_fold. econs 3; eauto. exists x. *)
-  (*     split; ss. punfold IND. auto. *)
-  (*   } *)
-  (*   { destruct LSIM0 as [LSIM IND]. eapply IH in IND. des. exists o. *)
-  (*     pfold. eapply pind9_fold. econs 4; eauto. *)
-  (*     split; ss. punfold IND. auto. *)
-  (*   } *)
-  (*   { destruct LSIM0 as [LSIM IND]. eapply IH in IND. des. exists o. *)
-  (*     pfold. eapply pind9_fold. econs 5; eauto. *)
-  (*     split; ss. punfold IND. auto. *)
-  (*   } *)
-  (*   { destruct LSIM0 as [LSIM IND]. eapply IH in IND. des. exists o. *)
-  (*     pfold. eapply pind9_fold. econs 6; eauto. *)
-  (*     split; ss. punfold IND. auto. *)
-  (*   } *)
-  (*   { exists (@ord_tree_base (A R0 R1)). *)
-  (*     pfold. eapply pind9_fold. econs 7; eauto. *)
-  (*   } *)
-  (*   { des. destruct LSIM as [LSIM IND]. eapply IH in IND. des. exists o. *)
-  (*     pfold. eapply pind9_fold. econs 8; eauto. esplits; eauto. *)
-  (*     split; ss. punfold IND. auto. *)
-  (*   } *)
-
-  (*   { destruct LSIM0 as [LSIM IND]. eapply IH in IND. des. exists o. *)
-  (*     pfold. eapply pind9_fold. econs 9; eauto. *)
-  (*     split; ss. punfold IND. auto. *)
-  (*   } *)
-
-  (*   { hexploit ord_tree_join. *)
-  (*     { instantiate (2:=A R0 R1). *)
-  (*       instantiate (2:= fun '(ps, pt, rs, src, tgt, shr) => (@rr R0 R1 LRR ps pt rs src tgt shr) /\ (ps = true)). *)
-  (*       i. ss. des_ifs. eapply IH in SAT. *)
-  (*       instantiate (1:= fun '(ps, pt, rs, src, tgt, shr) o => lsim wf_stt I tid (embed_lrr wf_stt LRR) ps pt rs (o, src) tgt shr). *)
-  (*       eauto. *)
-  (*     } *)
-  (*     intro JOIN. des. exists o1. pfold. eapply pind9_fold. econs 10. i. specialize (LSIM0 x). *)
-  (*     destruct LSIM0 as [LSIM IND]. *)
-  (*     specialize (JOIN (ps, true, r_ctx, src, (ktr_tgt x), (ths, im_src, im_tgt, st_src, st_tgt, r_shared))). des_ifs. *)
-  (*     eapply JOIN in IND; clear JOIN. des. *)
-  (*     split; ss. *)
-  (*     eapply stutter_lrr_ord_weak in IND. punfold IND. *)
-  (*     - i. unfold le in LE; des; clarify. unfold embed_lrr in *. des; split; eauto. *)
-  (*     - right; auto. *)
-  (*   } *)
-
-  (*   { destruct LSIM0 as [LSIM IND]. eapply IH in IND. des. exists o. *)
-  (*     pfold. eapply pind9_fold. econs 11; eauto. *)
-  (*     split; ss. punfold IND. *)
-  (*   } *)
-  (*   { destruct LSIM0 as [LSIM IND]. eapply IH in IND. des. exists o. *)
-  (*     pfold. eapply pind9_fold. econs 12; eauto. *)
-  (*     split; ss. punfold IND. *)
-  (*   } *)
-  (*   { destruct LSIM0 as [LSIM IND]. eapply IH in IND. des. exists o. *)
-  (*     pfold. eapply pind9_fold. econs 13; eauto. *)
-  (*     split; ss. punfold IND. *)
-  (*   } *)
-
-  (*   { hexploit ord_tree_join. *)
-  (*     { instantiate (2:=A R0 R1). *)
-  (*       instantiate (2:= fun '(ps, pt, rs, src, tgt, shr) => @rr R0 R1 LRR ps pt rs src tgt shr). *)
-  (*       i. ss. des_ifs. eapply IH in SAT. *)
-  (*       instantiate (1:= fun '(ps, pt, rs, src, tgt, shr) o => lsim wf_stt I tid (embed_lrr wf_stt LRR) ps pt rs (o, src) tgt shr). *)
-  (*       eauto. *)
-  (*     } *)
-  (*     intro JOIN. des. exists o1. pfold. eapply pind9_fold. econs 14. i. specialize (LSIM0 _ FAIR). *)
-  (*     destruct LSIM0 as [LSIM IND]. *)
-  (*     specialize (JOIN (ps, true, r_ctx, src, (ktr_tgt ()), (ths, im_src, im_tgt1, st_src, st_tgt, r_shared))). des_ifs. *)
-  (*     eapply JOIN in IND; clear JOIN. des. *)
-  (*     split; ss. *)
-  (*     eapply stutter_lrr_ord_weak in IND. punfold IND. *)
-  (*     - i. unfold le in LE; des; clarify. unfold embed_lrr in *. des; split; eauto. *)
-  (*     - right; auto. *)
-  (*   } *)
-
-  (*   { hexploit ord_tree_join. *)
-  (*     { instantiate (2:=A R0 R1). *)
-  (*       instantiate (2:= fun '(ps, pt, rs, src, tgt, shr) => @rr R0 R1 LRR ps pt rs src tgt shr). *)
-  (*       i. ss. des_ifs. eapply IH in SAT. *)
-  (*       instantiate (1:= fun '(ps, pt, rs, src, tgt, shr) o => lsim wf_stt I tid (embed_lrr wf_stt LRR) ps pt rs (o, src) tgt shr). *)
-  (*       eauto. *)
-  (*     } *)
-  (*     intro JOIN. des. exists o1. pfold. eapply pind9_fold. econs 15. i. specialize (LSIM0 ret). *)
-  (*     destruct LSIM0 as [LSIM IND]. *)
-  (*     specialize (JOIN (true, true, r_ctx, ktr_src ret, ktr_tgt ret, (ths, im_src, im_tgt, st_src, st_tgt, r_shared))). des_ifs. *)
-  (*     eapply JOIN in IND; clear JOIN. des. *)
-  (*     eapply stutter_lrr_ord_weak in IND. punfold IND. *)
-  (*     - i. unfold le in LE; des; clarify. unfold embed_lrr in *. des; split; eauto. *)
-  (*     - right; auto. *)
-  (*   } *)
-
-  (*   { hexploit ord_tree_join. *)
-  (*     { instantiate (2:=A R0 R1). *)
-  (*       instantiate (2:= fun '(ps, pt, rs, src, tgt, shr) => @rr R0 R1 LRR ps pt rs src tgt shr). *)
-  (*       i. ss. des_ifs. eapply IH in SAT. *)
-  (*       instantiate (1:= fun '(ps, pt, rs, src, tgt, shr) o => lsim wf_stt I tid (embed_lrr wf_stt LRR) ps pt rs (o, src) tgt shr). *)
-  (*       eauto. *)
-  (*     } *)
-  (*     intro JOIN. des. exists o1. pfold. eapply pind9_fold. econs 16; eauto. i. *)
-  (*     specialize (LSIM0 _ _ _ _ _ _ _ INV0 VALID0 _ TGT). *)
-  (*     destruct LSIM0 as [LSIM IND]. *)
-  (*     specialize (JOIN (ps, true, r_ctx1, (x <- trigger Yield;; ktr_src x), ktr_tgt (), (ths1, im_src1, im_tgt2, st_src1, st_tgt1, r_shared1))). des_ifs. *)
-  (*     eapply JOIN in IND; clear JOIN. des. esplits; eauto. *)
-  (*     left. eapply lsim_reset_prog. eauto. all: ss. *)
-  (*   } *)
-
-  (*   { des. destruct LSIM as [LSIM IND]. eapply IH in IND. des. exists o. *)
-  (*     pfold. eapply pind9_fold. econs 17; eauto. esplits; eauto. *)
-  (*     split; ss. punfold IND. *)
-  (*   } *)
 
   Lemma nosync_implies_stutter
         tid
@@ -307,7 +157,7 @@ Section PROOF.
         (LSIM: ModSimNoSync.lsim I tid LRR ps pt r_ctx src tgt shr)
     :
     exists (o: (@wf_stt R0 R1).(T)),
-      ModSimStutter.lsim wf_stt I tid (embed_lrr wf_stt LRR) ps pt r_ctx (o, src) tgt shr.
+      ModSimStutter.lsim wf_stt I tid LRR ps pt r_ctx (o, src) tgt shr.
   Proof.
     punfold LSIM.
     pattern R0, R1, LRR, ps, pt, r_ctx, src, tgt, shr.
@@ -319,8 +169,7 @@ Section PROOF.
 
     { remember (fun _: (A R0 R1) => @ord_tree_base (A R0 R1)) as ao. exists (ord_tree_cons ao).
       pfold. eapply pind9_fold. econs 1; eauto.
-      unfold embed_lrr. splits; auto. ss.
-      exists (ao (ps, pt, r_ctx, Ret r_src, Ret r_tgt, (ths, im_src, im_tgt, st_src, st_tgt, r_shared))).
+      instantiate (1:=ao (ps, pt, r_ctx, Ret r_src, Ret r_tgt, (ths, im_src, im_tgt, st_src, st_tgt, r_shared))).
       eapply ord_tree_lt_intro.
     }
 
@@ -361,7 +210,7 @@ Section PROOF.
       { instantiate (2:=A R0 R1).
         instantiate (2:= fun '(ps, pt, rs, src, tgt, shr) => @rr R0 R1 LRR ps pt rs src tgt shr).
         i. ss. des_ifs. eapply IH in SAT.
-        instantiate (1:= fun '(ps, pt, rs, src, tgt, shr) o => lsim wf_stt I tid (embed_lrr wf_stt LRR) ps pt rs (o, src) tgt shr).
+        instantiate (1:= fun '(ps, pt, rs, src, tgt, shr) o => lsim wf_stt I tid LRR ps pt rs (o, src) tgt shr).
         eauto.
       }
       intro JOIN. des. exists o1. pfold. eapply pind9_fold. econs 10. i. specialize (LSIM0 x).
@@ -369,9 +218,7 @@ Section PROOF.
       specialize (JOIN (ps, true, r_ctx, src, (ktr_tgt x), (ths, im_src, im_tgt, st_src, st_tgt, r_shared))). des_ifs.
       eapply JOIN in IND; clear JOIN. des.
       split; ss.
-      eapply stutter_lrr_ord_weak in IND. punfold IND.
-      - i. unfold le in LE; des; clarify. unfold embed_lrr in *. des; split; eauto.
-      - right; auto.
+      eapply stutter_ord_weak in IND. punfold IND. auto.
     }
 
     { destruct LSIM0 as [LSIM IND]. eapply IH in IND. des. exists o.
@@ -391,7 +238,7 @@ Section PROOF.
       { instantiate (2:=A R0 R1).
         instantiate (2:= fun '(ps, pt, rs, src, tgt, shr) => @rr R0 R1 LRR ps pt rs src tgt shr).
         i. ss. des_ifs. eapply IH in SAT.
-        instantiate (1:= fun '(ps, pt, rs, src, tgt, shr) o => lsim wf_stt I tid (embed_lrr wf_stt LRR) ps pt rs (o, src) tgt shr).
+        instantiate (1:= fun '(ps, pt, rs, src, tgt, shr) o => lsim wf_stt I tid LRR ps pt rs (o, src) tgt shr).
         eauto.
       }
       intro JOIN. des. exists o1. pfold. eapply pind9_fold. econs 14. i. specialize (LSIM0 _ FAIR).
@@ -399,32 +246,28 @@ Section PROOF.
       specialize (JOIN (ps, true, r_ctx, src, (ktr_tgt ()), (ths, im_src, im_tgt1, st_src, st_tgt, r_shared))). des_ifs.
       eapply JOIN in IND; clear JOIN. des.
       split; ss.
-      eapply stutter_lrr_ord_weak in IND. punfold IND.
-      - i. unfold le in LE; des; clarify. unfold embed_lrr in *. des; split; eauto.
-      - right; auto.
+      eapply stutter_ord_weak in IND. punfold IND. auto.
     }
 
     { hexploit ord_tree_join.
       { instantiate (2:=A R0 R1).
         instantiate (2:= fun '(ps, pt, rs, src, tgt, shr) => @rr R0 R1 LRR ps pt rs src tgt shr).
         i. ss. des_ifs. eapply IH in SAT.
-        instantiate (1:= fun '(ps, pt, rs, src, tgt, shr) o => lsim wf_stt I tid (embed_lrr wf_stt LRR) ps pt rs (o, src) tgt shr).
+        instantiate (1:= fun '(ps, pt, rs, src, tgt, shr) o => lsim wf_stt I tid LRR ps pt rs (o, src) tgt shr).
         eauto.
       }
       intro JOIN. des. exists o1. pfold. eapply pind9_fold. econs 15. i. specialize (LSIM0 ret).
       destruct LSIM0 as [LSIM IND].
       specialize (JOIN (true, true, r_ctx, ktr_src ret, ktr_tgt ret, (ths, im_src, im_tgt, st_src, st_tgt, r_shared))). des_ifs.
       eapply JOIN in IND; clear JOIN. des.
-      eapply stutter_lrr_ord_weak in IND. punfold IND.
-      - i. unfold le in LE; des; clarify. unfold embed_lrr in *. des; split; eauto.
-      - right; auto.
+      eapply stutter_ord_weak in IND. punfold IND. auto.
     }
 
     { hexploit ord_tree_join.
       { instantiate (2:=A R0 R1).
         instantiate (2:= fun '(ps, pt, rs, src, tgt, shr) => @rr R0 R1 LRR ps pt rs src tgt shr).
         i. ss. des_ifs. eapply IH in SAT.
-        instantiate (1:= fun '(ps, pt, rs, src, tgt, shr) o => lsim wf_stt I tid (embed_lrr wf_stt LRR) ps pt rs (o, src) tgt shr).
+        instantiate (1:= fun '(ps, pt, rs, src, tgt, shr) o => lsim wf_stt I tid LRR ps pt rs (o, src) tgt shr).
         eauto.
       }
       intro JOIN. des. exists o1. pfold. eapply pind9_fold. econs 16; eauto. i.
@@ -440,231 +283,9 @@ Section PROOF.
       split; ss. punfold IND.
     }
 
-    (*TODO*)
-
-
-
-    
-    pclearbot. rename LSIM0 into LSIM. punfold LSIM.
-    eapply pind9_unfold in LSIM.
-    2:{ eapply ModSimNoSync._lsim_mon. }
-    inv LSIM.
-
-    { remember (fun _: (A R0 R1) => @ord_tree_base (A R0 R1)) as ao. exists (ord_tree_cons ao).
-      pfold. eapply pind9_fold. econs 1; eauto.
-      unfold embed_lrr. splits; auto. ss.
-      exists (ao (false, false, r_ctx, Ret r_src, Ret r_tgt, (ths, im_src, im_tgt, st_src, st_tgt, r_shared))).
-      eapply ord_tree_lt_intro.
-    }
-
-    { destruct LSIM0 as [LSIM IND]. eapply IH in IND. des. exists o.
-      pfold. eapply pind9_fold. econs 2; eauto.
-      split; ss. punfold IND.
-    }
-    { des. destruct LSIM0 as [LSIM IND]. eapply IH in IND. des. exists o.
-      pfold. eapply pind9_fold. econs 3; eauto. exists x.
-      split; ss. punfold IND.
-    }
-    { destruct LSIM0 as [LSIM IND]. eapply IH in IND. des. exists o.
-      pfold. eapply pind9_fold. econs 4; eauto.
-      split; ss. punfold IND.
-    }
-    { destruct LSIM0 as [LSIM IND]. eapply IH in IND. des. exists o.
-      pfold. eapply pind9_fold. econs 5; eauto.
-      split; ss. punfold IND.
-    }
-    { destruct LSIM0 as [LSIM IND]. eapply IH in IND. des. exists o.
-      pfold. eapply pind9_fold. econs 6; eauto.
-      split; ss. punfold IND.
-    }
-    { exists (@ord_tree_base (A R0 R1)).
-      pfold. eapply pind9_fold. econs 7; eauto.
-    }
-    { des. destruct LSIM as [LSIM IND]. eapply IH in IND. des. exists o.
-      pfold. eapply pind9_fold. econs 8; eauto. esplits; eauto.
-      split; ss. punfold IND.
-    }
-
-    { destruct LSIM0 as [LSIM IND]. eapply IH in IND. des. exists o.
-      pfold. eapply pind9_fold. econs 9; eauto.
-      split; ss. punfold IND.
-    }
-
-    { hexploit ord_tree_join.
-      { instantiate (2:=A R0 R1).
-        instantiate (2:= fun '(ps, pt, rs, src, tgt, shr) => @rr R0 R1 LRR ps pt rs src tgt shr).
-        i. ss. des_ifs. eapply IH in SAT.
-        instantiate (1:= fun '(ps, pt, rs, src, tgt, shr) o => lsim wf_stt I tid (embed_lrr wf_stt LRR) ps pt rs (o, src) tgt shr).
-        eauto.
-      }
-      intro JOIN. des. exists o1. pfold. eapply pind9_fold. econs 10. i. specialize (LSIM0 x).
-      destruct LSIM0 as [LSIM IND].
-      specialize (JOIN (ps, true, r_ctx, src, (ktr_tgt x), (ths, im_src, im_tgt, st_src, st_tgt, r_shared))). des_ifs.
-      eapply JOIN in IND; clear JOIN. des.
-      split; ss.
-      eapply stutter_lrr_ord_weak in IND. punfold IND.
-      - i. unfold le in LE; des; clarify. unfold embed_lrr in *. des; split; eauto.
-      - right; auto.
-    }
-
-    { destruct LSIM0 as [LSIM IND]. eapply IH in IND. des. exists o.
-      pfold. eapply pind9_fold. econs 11; eauto.
-      split; ss. punfold IND.
-    }
-    { destruct LSIM0 as [LSIM IND]. eapply IH in IND. des. exists o.
-      pfold. eapply pind9_fold. econs 12; eauto.
-      split; ss. punfold IND.
-    }
-    { destruct LSIM0 as [LSIM IND]. eapply IH in IND. des. exists o.
-      pfold. eapply pind9_fold. econs 13; eauto.
-      split; ss. punfold IND.
-    }
-
-    { hexploit ord_tree_join.
-      { instantiate (2:=A R0 R1).
-        instantiate (2:= fun '(ps, pt, rs, src, tgt, shr) => @rr R0 R1 LRR ps pt rs src tgt shr).
-        i. ss. des_ifs. eapply IH in SAT.
-        instantiate (1:= fun '(ps, pt, rs, src, tgt, shr) o => lsim wf_stt I tid (embed_lrr wf_stt LRR) ps pt rs (o, src) tgt shr).
-        eauto.
-      }
-      intro JOIN. des. exists o1. pfold. eapply pind9_fold. econs 14. i. specialize (LSIM0 _ FAIR).
-      destruct LSIM0 as [LSIM IND].
-      specialize (JOIN (ps, true, r_ctx, src, (ktr_tgt ()), (ths, im_src, im_tgt1, st_src, st_tgt, r_shared))). des_ifs.
-      eapply JOIN in IND; clear JOIN. des.
-      split; ss.
-      eapply stutter_lrr_ord_weak in IND. punfold IND.
-      - i. unfold le in LE; des; clarify. unfold embed_lrr in *. des; split; eauto.
-      - right; auto.
-    }
-
-    { hexploit ord_tree_join.
-      { instantiate (2:=A R0 R1).
-        instantiate (2:= fun '(ps, pt, rs, src, tgt, shr) => @rr R0 R1 LRR ps pt rs src tgt shr).
-        i. ss. des_ifs. eapply IH in SAT.
-        instantiate (1:= fun '(ps, pt, rs, src, tgt, shr) o => lsim wf_stt I tid (embed_lrr wf_stt LRR) ps pt rs (o, src) tgt shr).
-        eauto.
-      }
-      intro JOIN. des. exists o1. pfold. eapply pind9_fold. econs 15. i. specialize (LSIM0 ret).
-      destruct LSIM0 as [LSIM IND].
-      specialize (JOIN (true, true, r_ctx, ktr_src ret, ktr_tgt ret, (ths, im_src, im_tgt, st_src, st_tgt, r_shared))). des_ifs.
-      eapply JOIN in IND; clear JOIN. des.
-      eapply stutter_lrr_ord_weak in IND. punfold IND.
-      - i. unfold le in LE; des; clarify. unfold embed_lrr in *. des; split; eauto.
-      - right; auto.
-    }
-
-    { hexploit ord_tree_join.
-      { instantiate (2:=A R0 R1).
-        instantiate (2:= fun '(ps, pt, rs, src, tgt, shr) => @rr R0 R1 LRR ps pt rs src tgt shr).
-        i. ss. des_ifs. eapply IH in SAT.
-        instantiate (1:= fun '(ps, pt, rs, src, tgt, shr) o => lsim wf_stt I tid (embed_lrr wf_stt LRR) ps pt rs (o, src) tgt shr).
-        eauto.
-      }
-      intro JOIN. des. exists o1. pfold. eapply pind9_fold. econs 16; eauto. i.
-      specialize (LSIM0 _ _ _ _ _ _ _ INV0 VALID0 _ TGT).
-      destruct LSIM0 as [LSIM IND].
-      specialize (JOIN (ps, true, r_ctx1, (x <- trigger Yield;; ktr_src x), ktr_tgt (), (ths1, im_src1, im_tgt2, st_src1, st_tgt1, r_shared1))). des_ifs.
-      eapply JOIN in IND; clear JOIN. des. esplits; eauto.
-      left. eapply lsim_reset_prog. eauto. all: ss.
-    }
-
-    { des. destruct LSIM as [LSIM IND]. eapply IH in IND. des. exists o.
-      pfold. eapply pind9_fold. econs 17; eauto. esplits; eauto.
-      split; ss. punfold IND.
-    }
-
+    { exists (@ord_tree_base _). pfold. eapply pind9_fold. econs 18. pclearbot. auto. }
 
   Qed.
-
-
-  (* Theorem nosync_implies_stutter *)
-  (*         tid *)
-  (*         R0 R1 (RR: RR_rel R0 R1) *)
-  (*         ps pt r_ctx src tgt *)
-  (*         (shr: shared) *)
-  (*         (LSIM: ModSimNoSync.lsim I tid RR ps pt r_ctx src tgt shr) *)
-  (*   : *)
-  (*   exists o, ModSimStutter.lsim (@ord_tree_WF (A R0 R1)) I tid RR ps pt r_ctx (o, src) tgt shr. *)
-  (* Proof. *)
-  (*   revert_until tid. pcofix CIH; i. *)
-  (*   punfold LSIM. *)
-  (*   pattern R0, R1, RR, ps, pt, r_ctx, src, tgt, shr. *)
-  (*   revert R0 R1 RR ps pt r_ctx src tgt shr LSIM. apply pind9_acc. *)
-  (*   intros rr DEC IH. clear DEC. intros R0 R1 RR ps pt r_ctx src tgt shr LSIM. *)
-  (*   eapply pind9_unfold in LSIM. *)
-  (*   2:{ eapply ModSimNoSync._lsim_mon. } *)
-  (*   inv LSIM. *)
-
-  (*   { pfold. eapply pind9_fold. econs 1; eauto. } *)
-  (*   { pfold. eapply pind9_fold. econs 2; eauto. *)
-  (*     split; ss. destruct LSIM0 as [LSIM IND]. eapply IH in IND. punfold IND. *)
-  (*   } *)
-  (*   { pfold. eapply pind9_fold. econs 3; eauto. *)
-  (*     des. exists x. *)
-  (*     split; ss. destruct LSIM0 as [LSIM IND]. eapply IH in IND. punfold IND. *)
-  (*   } *)
-  (*   { pfold. eapply pind9_fold. econs 4; eauto. *)
-  (*     split; ss. destruct LSIM0 as [LSIM IND]. eapply IH in IND. punfold IND. *)
-  (*   } *)
-  (*   { pfold. eapply pind9_fold. econs 5; eauto. *)
-  (*     split; ss. destruct LSIM0 as [LSIM IND]. eapply IH in IND. punfold IND. *)
-  (*   } *)
-  (*   { pfold. eapply pind9_fold. econs 6; eauto. *)
-  (*     split; ss. destruct LSIM0 as [LSIM IND]. eapply IH in IND. punfold IND. *)
-  (*   } *)
-  (*   { pfold. eapply pind9_fold. econs 7; eauto. } *)
-  (*   { pfold. eapply pind9_fold. econs 8; eauto. *)
-  (*     des. esplits; eauto. *)
-  (*     split; ss. destruct LSIM as [LSIM IND]. eapply IH in IND. punfold IND. *)
-  (*   } *)
-  (*   { pfold. eapply pind9_fold. econs 9; eauto. *)
-  (*     split; ss. destruct LSIM0 as [LSIM IND]. eapply IH in IND. punfold IND. *)
-  (*   } *)
-  (*   { pfold. eapply pind9_fold. econs 10; eauto. *)
-  (*     i. specialize (LSIM0 x). *)
-  (*     split; ss. destruct LSIM0 as [LSIM IND]. eapply IH in IND. punfold IND. *)
-  (*   } *)
-  (*   { pfold. eapply pind9_fold. econs 11; eauto. *)
-  (*     split; ss. destruct LSIM0 as [LSIM IND]. eapply IH in IND. punfold IND. *)
-  (*   } *)
-  (*   { pfold. eapply pind9_fold. econs 12; eauto. *)
-  (*     split; ss. destruct LSIM0 as [LSIM IND]. eapply IH in IND. punfold IND. *)
-  (*   } *)
-  (*   { pfold. eapply pind9_fold. econs 13; eauto. *)
-  (*     split; ss. destruct LSIM0 as [LSIM IND]. eapply IH in IND. punfold IND. *)
-  (*   } *)
-  (*   { pfold. eapply pind9_fold. econs 14; eauto. *)
-  (*     i. specialize (LSIM0 _ FAIR). *)
-  (*     split; ss. destruct LSIM0 as [LSIM IND]. eapply IH in IND. punfold IND. *)
-  (*   } *)
-  (*   { pfold. eapply pind9_fold. econs 15; eauto. *)
-  (*     i. specialize (LSIM0 ret). pclearbot. *)
-  (*     right. eapply CIH; eauto. *)
-  (*   } *)
-
-  (*   { pfold. eapply pind9_fold. eapply ModSimNoSync.lsim_yieldL. *)
-  (*     des. esplits; eauto. *)
-  (*     split; ss. destruct LSIM as [LSIM IND]. eapply IH in IND. punfold IND. *)
-  (*   } *)
-
-  (*   { pfold. eapply pind9_fold. eapply ModSimNoSync.lsim_yieldR; eauto. *)
-  (*     i. specialize (LSIM0 _ _ _ _ _ _ _ INV0 VALID0 _ TGT). *)
-  (*     split; ss. destruct LSIM0 as [LSIM IND]. eapply IH in IND. punfold IND. *)
-  (*   } *)
-
-  (*   { pfold. eapply pind9_fold. eapply ModSimNoSync.lsim_yieldR; eauto. *)
-  (*     i. specialize (LSIM0 _ _ _ _ _ _ _ INV0 VALID0 _ TGT). *)
-  (*     split; ss. eapply pind9_fold. eapply ModSimNoSync.lsim_yieldL. *)
-  (*     des. esplits. eapply FAIR. split; ss. pclearbot. *)
-  (*     eapply pind9_fold. eapply ModSimNoSync.lsim_progress. right. *)
-  (*     eapply CIH. apply ModSimStid.lsim_set_prog; auto. *)
-  (*   } *)
-
-  (*   { pfold. eapply pind9_fold. eapply ModSimNoSync.lsim_progress. right. *)
-  (*     eapply CIH. pclearbot. auto. *)
-  (*   } *)
-
-  (* Qed. *)
 
 End PROOF.
 
